separated seqext.fst into an interface and proof file.

src/specs/seqext.fsi
@@ -1,0 +1,104 @@
+(*--build-config
+   options:--admit_fsi Seq;
+   other-files:seq.fsi
+--*)
+
+// $legal:614:
+//
+// Copyright 2015 Michael Lowell Roberts
+//
+// Licensed under the Apache License, Version 2.0 (the "License");
+// you may not use this file except in compliance with the License.
+// You may obtain a copy of the License at
+//
+//     http://www.apache.org/licenses/LICENSE-2.0
+//
+// Unless required by applicable law or agreed to in writing, software
+// distributed under the License is distributed on an "AS IS" BASIS,
+// WITHOUT WARRANTIES OR CONDITIONS OF ANY KIND, either express or implied.
+// See the License for the specific language governing permissions and
+// limitations under the License.
+//
+// ,$
+
+module Tesseract.Specs.SeqExt
+   open Seq
+
+   val filter:
+      // predicate; if false, then the element is discarded from the sequence.
+      ('a -> Tot bool)
+      // input sequence
+      -> seq 'a
+      // output sequence
+      -> Tot (seq 'a)
+
+   val lemma_filter__length:
+      p: ('a -> Tot bool) ->
+      s: seq 'a ->
+      Lemma
+         (requires True)
+         (ensures (length (filter p s) <= length s))
+         [SMTPat (length (filter p s))]
+
+   val lemma_filter__contents:
+      p: ('a -> Tot bool) ->
+      s: seq 'a ->
+      Lemma
+         (requires True)
+         (ensures
+            (forall i.
+               0 <= i && i < length (filter p s)
+               ==> p (index (filter p s) i)))
+
+   val insert:
+      s: seq 'a
+      -> i: nat{i <= length s}
+      -> 'a
+      -> Tot (seq 'a)
+
+   val lemma_insert__length:
+      s: seq 'a
+      -> i: nat{i <= length s}
+      -> a: 'a
+      -> Lemma
+         (requires True)
+         (ensures (length (insert s i a) = length s + 1))
+         [SMTPat (length (insert s i a))]
+
+   val lemma_insert__contents:
+      s: seq 'a
+      -> i: nat{i <= length s}
+      -> a: 'a
+      -> Lemma
+         (ensures
+            (index (insert s i a) i = a
+            /\ (forall j. 0 <= j && j < i
+               ==> index (insert s i a) j = index s j)
+            /\ (forall j. i < j && j < length (insert s i a)
+               ==> index (insert s i a) j = index s (j - 1))))
+
+   val remove:
+      s: seq 'a{length s > 0}
+      -> i: nat{i < length s}
+      -> 'a
+      -> Tot (seq 'a)
+
+   val lemma_remove__length:
+      s: seq 'a{length s > 0}
+      -> i: nat{i < length s}
+      -> a: 'a
+      -> Lemma
+         (requires True)
+         (ensures (length (remove s i a) = length s - 1))
+         [SMTPat (length (remove s i a))]
+
+   val lemma_remove__contents:
+      s: seq 'a{length s > 0}
+      -> i: nat{i < length s}
+      -> a: 'a
+      -> Lemma
+         (ensures
+            ((forall j. 0 <= j && j < i
+               ==> index (remove s i a) j = index s j)
+            /\ (forall j. i <= j && j < length (remove s i a)
+               ==> index (remove s i a) j = index s (j + 1))))
